src/Std/Data/TreeMap/Raw.lean
@@ -120,7 +120,7 @@ def insertIfNew (t : Raw α β cmp) (a : α) (b : β) : Raw α β cmp :=
     letI : Ord α := ⟨cmp⟩; ⟨t.inner.insertIfNew a b⟩
 
 @[inline, inherit_doc DTreeMap.Raw.containsThenInsertIfNew]
-def containsThenInsertIfNew [BEq α] [Hashable α] (t : Raw α β cmp) (a : α) (b : β) :
+def containsThenInsertIfNew (t : Raw α β cmp) (a : α) (b : β) :
     Bool × Raw α β cmp :=
   let p := t.inner.containsThenInsertIfNew a b
   (p.1, ⟨p.2⟩)
