src/Std/Data/TreeSet/Basic.lean
@@ -100,7 +100,7 @@ def insertIfNew (t : TreeSet α cmp) (a : α) : TreeSet α cmp :=
   ⟨t.inner.insertIfNew a ()⟩
 
 @[inline, inherit_doc Raw.containsThenInsertIfNew]
-def containsThenInsertIfNew [BEq α] [Hashable α] (t : TreeSet α cmp) (a : α) :
+def containsThenInsertIfNew (t : TreeSet α cmp) (a : α) :
     Bool × TreeSet α cmp :=
   let p := t.inner.containsThenInsertIfNew a ()
   (p.1, ⟨p.2⟩)
